\documentclass[12pt,a4paper]{book}

\input{../../template/standard_pkgs}
\input{../../template/common}
\input{format}

\theoremstyle{plain}
\newtheorem*{pro}{\cmss\problemColor Problem}
\addto\captionsvietnam{\renewcommand{\proofname}{\cmss\problemColor Proof}}

\begin{document}

\begin{pro}
Let $a,\,b,\,c$ be positive numbers and $x,\,y,\,z$  be the lengths of the sides of a triangle. Prove that
\[a(y+z-x)+b(z+x-y)+c(x+y-z) \geq \frac{(x+y+z)(xbc+yca+zab)}{ax+by+cz}.\]
\begin{flushright}(Nguyen Van Huyen)\end{flushright}
\end{pro}

\begin{proof}
% (\textit{Michael Rozenberg}) 
Using Ravi's substitution, we need to prove that
\begin{equation}\label{eq1}
ax+by+cz\geq\frac{(x+y+z)[ab(x+y)+bc(y+z)+ca(z+x)]}{a(y+z)+b(x+z)+c(x+y)},
\end{equation}
where $x$, $y$ and $z$ are positive numbers.

We write the inequality \eqref{eq1} as
$$f(c) = z(x+y)c^2-2z(xa+yb)c+x(y+z)a^2-2xyab+y(x+z)b^2 \geq 0.$$
The quadratic $f(c)$ has the discriminant
\[\begin{aligned}
\Delta_c &= z(xa+yb)^2-(x+y)[x(y+z)a^2-2xyab+y(x+z)b^2] \\&
= - xy(x+y+z)a^2 - xy(x+y+z)b^2 + 2abxy(x+y+z) \\&
% = - (x+y+z)[xy(x+y+z)a^2 - xy(x+y+z)b^2 + 2abxy(x+y+z)] \\&
= - xy(x+y+z)(a-b)^2 \leqslant 0.
\end{aligned}\]
%$$[x(x+y)(x+z)-x^2z]a^2+[y(y+x)(y+z)-y^2z]b^2 \geq 2xy(x+y+z)ab,$$
%Which is true by AM-GM and Cauchy-Schwarz inequality, we have
%$$(x(x+y)(x+z)-x^2z)a^2+(y(y+x)(y+z)-y^2z)b^2\geq2\sqrt{(x(x+y)(x+z)-x^2z)\cdot(y(y+x)(y+z)-y^2z)}ab=$$
%$$=2\sqrt{xy(x^2+xy+yz)(xy+y^2+xz)}ab\geq2\sqrt{xy\cdot xy(x+y+z)^2}ab=2xy(x+y+z)ab.$$
Thus, $f(c) \ge 0.$ The proof is completed.
\end{proof}

\begin{remark}
We have
\[\begin{aligned}
a(y&+z-x)+b(z+x-y)+c(x+y-z) - \frac{(x+y+z)(xbc+yca+zab)}{ax+by+cz} \\&
=\frac{[z^2-(x-y)^2](a-b)^2+[x^2-(y-z)^2](b-c)^2+[y^2-(z-x)^2](c-a)^2}{2(ax+by+cz)} \ge 0
\end{aligned}\]
\end{remark}

\begin{remark} $\,$
\begin{enumerate}[(1)]
\item If $a=y,\,b=z,\,c=x$ the inequality becomes
\[x^2y(x-y) + y^2z(y-z) + z^2x(z-x) \ge 0.\]
This is problem $6$ in the IMO $1983.$
\item If $a=x,\,b=y,\,c=z$ the inequality becomes
\[2(xy+yz+zx) \geqslant x^2+y^2+z^2+\frac{3xyz(x+y+z)}{x^2+y^2+z^2}.\]
\end{enumerate}
\end{remark}


\end{document}
