\documentclass[12pt,a4paper]{book}

\input{./template/standard_pkgs}
\input{./template/format}
\input{./template/define}

\begin{document}

\begin{pro_no_count}
Let $a, \,b,\,c$ be positive real numbers such that $a+b+c=3.$ Prove that
$$\dfrac{a(b+c)}{a^2+2bc+3} + \dfrac{b(c+a)}{b^2+2ca+3} + \dfrac{c(a+b)}{c^2+2ab+3} \le 1.$$
\end{pro_no_count}

\begin{proof}
%We have the following estimate
%$$\frac{a(b+c)}{a^2+2bc+\frac{(a+b+c)^2}{3}} \leq \frac{a(b+c)}{2(ab+bc+ca)}.$$
%Indeed, equivalent to
%$$3(a^2+2bc)+(a+b+c)^2 \geqslant 6(ab+bc+ca),$$
%or
%$$4a^2+(b+c)^2 \geqslant 4a(b+c).$$
%Which is true by the AM-GM inequality
%$$4a^2+(b+c)^2 \geqslant 2\sqrt{4a^2 \cdot (b+c)^2} = 4a(b+c).$$
%Therefore
%$$\sum \frac{a(b+c)}{a^2+2bc+\frac{(a+b+c)^2}{3}} \leq \sum \frac{a(b+c)}{2(ab+bc+ca)} = 1.$$
%The proof is completed.
\textit{(Nguyen Van Huyen)} Using the Cauchy-Schwarz inequality and AM-GM inequality, we have
$$\begin{aligned}
a^2 + 3 = a^2+\frac{(a+b+c)^2}{3} \geqslant \frac{(a+a+b+c)^2}{1+3}  = \frac{(2a+b+c)^2}{4} \geqslant 2a(b+c).
\end{aligned}$$
So
$$a^2+2bc+3 \geqslant 2(ab+bc+ca),$$
or
$$\frac{a(b+c)}{a^2+2bc+3} \leq \frac{a(b+c)}{2(ab+bc+ca)}.$$
Therefore
$$\sum \frac{a(b+c)}{a^2+2bc+3} \leq \sum \frac{a(b+c)}{2(ab+bc+ca)} =1.$$
The proof is completed.
\end{proof}


\end{document}
