\documentclass[12pt,a4paper]{book}

\input{./template/standard_pkgs}
\input{./template/format}
\input{./template/define}

\begin{document}

\begin{pro_no_count}[Vasile Cirtoaje]
If $a,\,b,\,c$ are positive real numbers, then
\begin{equation}\label{eq_w8a6k}
\frac{a^2}{a^2+ab+b^2} + \frac{b^2}{b^2+bc+c^2} + \frac{c^2}{c^2+ca+a^2} \ge 1.
\end{equation} 
\end{pro_no_count}

\begin{proof}
(\textit{Nguyen Van Huyen}) Since
\[\sum \dfrac{a(ab-c^2)}{a+b+c} = 0,\]
and
\[\sum \frac{b^2+ab}{a^2+b^2+c^2+ab+bc+ca} = 1.\]
% We have the following estimate
We see that the inequality \eqref{eq_w8a6k} follows by adding the inequality below and two similar inequalities
\begin{equation}\label{eq02042005124}
\frac{b^2}{b^2+bc+c^2} \ge \frac{b^2+ab+\dfrac{a(ab-c^2)}{a+b+c}}{a^2+b^2+c^2+ab+bc+ca}.
\end{equation}
Indeed, we can rewrite the inequality \eqref{eq02042005124} as
\[\frac{b^2}{b^2+bc+c^2} -  \frac{b^2+ab}{a^2+b^2+c^2+ab+bc+ca} \ge \frac{\dfrac{a(ab-c^2)}{a+b+c}}{a^2+b^2+c^2+ab+bc+ca},\]
or
\[\frac{ab(ab-c^2)}{b^2+bc+c^2} \ge \frac{a(ab-c^2)}{a+b+c},\]
which is equivalent to
\[\frac{a(ab-c^2)^2}{(a+b+c)(b^2+bc+c^2)} \ge 0.\]
Thus, the inequality \eqref{eq02042005124} is proven.
%
%Thus
%\[\sum \frac{b^2}{b^2+bc+c^2} \ge \sum \frac{b^2+ab+\dfrac{a(ab-c^2)}{a+b+c}}{a^2+b^2+c^2+ab+bc+ca} = \sum \frac{b^2+ab}{a^2+b^2+c^2+ab+bc+ca} = 1.\]
\end{proof}

\end{document}
