\documentclass[12pt,a4paper]{book}

\input{../../template/standard_pkgs}
\input{../../template/common}
\input{format}

\theoremstyle{plain}
\newtheorem*{pro}{\cmss\problemColor Problem}

\addto\captionsvietnam{\renewcommand{\proofname}{\cmss\problemColor Proof}}

\begin{document}
\begin{pro}
Let $a,\,b,\,c$ be non-negative real numbers. Prove that
\begin{equation}\label{eq0}
a^3+b^3+c^3+2(ab^2+bc^2+ca^2) \geqslant 3(a^2b+b^2c+c^2a).
\end{equation}
\end{pro}

\begin{proof}[\cmss\problemColor Solution 1]
Note that
\[a^2b+b^2c+c^2a-3abc = c(a-b)^2 + a(a-c)(b-c),\]
\[a^3+b^3+c^3-3abc=(a+b+c)[(a-b)^2+(a-c)(b-c)].\]
Write the inequality \eqref{eq0} as
\[a^3+b^3+c^3-3abc+2(ab^2+bc^2+ca^2-3abc) \ge 3(a^2b+b^2c+c^2a-3abc).\]
or
\[(a+b)(a-b)^2 + (c+3b-2a)(a-c)(b-c) \geqslant 0.\]
Suppose \( c \) is between \( a \) and \( b \), then $(a-c)(c-b) \ge 0.$ By the AM-GM inequality, we have
$$(a-b)^2=[(a-c)+(c-b)]^2 \ge 4(a-c)(c-b).$$
So, we need to show that
\[4(a+b)(a-c)(c-b) + (c+3b-2a)(a-c)(b-c) \geqslant 0.\]
or
\begin{equation}\label{eq1}
(a-c)(c-b)(6a+b-c) \ge 0.
\end{equation} 
Now
\begin{enumerate}[\textbullet]
\item  If $a \geqslant c,$ then $6a+b-c = (a-c)+5a+b\ge0.$
\item  If $b \geqslant c,$ then $6a+b-c = (b-c)+6a \ge 0.$
\end{enumerate}
Therefore, \eqref{eq1} is always true. The proof is complete.
\end{proof}

{\cmss\problemColor Note.} In addition, we also have
\[c(6a+b-c) = (a-c)(c-b)+a(b+5c) \ge 0.\]

\begin{proof}[\cmss\problemColor Solution 2] 
Suppose $c=\min\{a,b,c\}.$ Let 
$a=x+c,$ $b=y+c $ for $x,y \ge 0.$ 

The inequality \eqref{eq0} become
\begin{equation}\label{eq2}
2(x^2-xy+y^2)c+x^3-3x^2y+2xy^2+y^3 \geqslant 0.
\end{equation}
But
\[x^3-3x^2y+2xy^2+y^3 = x(x-2y)^2+y(x-y)^2 \ge 0.\]
Therefore, \eqref{eq2} is always true.
\end{proof}


\end{document}
