\documentclass[12pt,a4paper]{book}

\input{../template/standard_pkgs}
\input{../template/common}
\input{format}

\addto\captionsvietnam{\renewcommand{\proofname}{\cmss\problemColor Proof}}

\begin{document}
\begin{pro}
Let $a,\,b,\,c$ are positive real numbers. Prove that
\[\frac{a^2}{b}+\frac{b^2}{c}+\frac{c^2}{a} \ge 3\sqrt[6]{\frac{a^6+b^6+c^6}{3}}.\]
\vspace{-1.3cm}
\begin{flushright}(Vo Quoc Ba Can)\end{flushright}
\end{pro}

\begin{proof}
(\textit{Nguyen Van Huyen}) We write the inequality as
\[\left(\frac{a^2}{b}+\frac{b^2}{c}+\frac{c^2}{a}\right)^6 \ge 243(a^6+b^6+c^6).\]
WLOG, suppose $a+b+c=1,$ setting $q=\frac{1-t^2}{3}$ with $0 \le t < 1, $ we have
\[a^6+b^6+c^6=3r^2+6p(p^2-2q)r+(p^2-2q)(p^4-4p^2q+q^2)\]
\[=3r^2+2(2t^2+1)r+\frac{1}{27}(2t^2+1)(t^4+10t^2-2).\]
In addition, from \footnote{\url{https://wp.me/p7ChCZ-ht}}
\[0 < r \leqslant r_0 = \frac{p(9q-2p^2)+2(p^2-3q)\sqrt{p^2-3q}}{27},\]
with $q=\frac{1-t^2}{3},$ we get
\[0 < r \leqslant r_0 = \frac{(1+2t)(1-t)^2}{27}.\]
so
\[243(a^6+b^6+c^6) \leqslant 243\left[3r_0^2+2(2t^2+1)r_0+\frac{1}{27}(2t^2+1)(t^4+10t^2-2)\right]\]
\[=(2t+1)^2(1-t)^4+18(2t^2+1)(2t+1)(1-t)^2+9(2t^2+1)(t^4+10t^2-2)\]
\[=22t^6+60t^5+90t^4+40t^3+30t^2+1.\]
We need to prove
\[\left(\frac{a^2}{b}+\frac{b^2}{c}+\frac{c^2}{a}\right)^6 \ge 22t^6+60t^5+90t^4+40t^3+30t^2+1,\]
Using the inequality (\textit{lemma $2$}) \footnote{\url{https://wp.me/p7ChCZ-ZS}}
\[\frac{a^2}{b}+\frac{b^2}{c}+\frac{c^2}{a} \ge \frac{1+2t+5t^2+4t^3-3t^4}{(2t+1)(1-t^2)},\]
we will show that
\[\left(\frac{1+2t+5t^2+4t^3-3t^4}{(2t+1)(1-t^2)}\right)^6 \ge 22t^6+60t^5+90t^4+40t^3+30t^2+1,\]
equivalent to
\[(1+2t+5t^2+4t^3-3t^4)^6 \ge (22t^6+60t^5+90t^4+40t^3+30t^2+1)(2t+1)^6(1-t^2)^6,\]
or
\[t^2 \cdot f(t) \geq 0,\]
for
\[\begin{aligned}
f(t) = & \; 6-4t-48t^2+1620t^3+14278t^4+56208t^5
\\&+131769t^6+197148t^7+177936t^8+59148t^9-50214t^{10}
\\&-25188t^{11}+69318t^{12}+40416t^{13}-98436t^{14}-118368t^{15}-1320t^{16}
\\&+46524t^{17}+25437t^{18}+21748t^{19}-1962t^{20}-13896t^{21}-679t^{22}.
\end{aligned}\]
We will show that $f(t) >0.$ Indeed, setting $t = \frac{1}{x+1} < 1$ with $x>0,$ we have
\[f(t) = f\left(\frac{1}{x+1}\right)  = \frac{g(x)}{(x+1)^{22}},\]
with
\[\begin{aligned}
g(x) = & \; 6x^{22}+128x^{21}+1254x^{20}+9060x^{19}+74508x^{18}+669576x^{17}
\\&+4975341x^{16}+27941724x^{15}
+119289936x^{14}+395553816x^{13}\\&+1037590858x^{12}+2180644272x^{11}+3699912978x^{10}
+5084994888x^9\\&+5658046506x^8+5075026812x^7+3637113678x^6
+2051467236x^5\\&+888549669x^4+283986324x^3+62710038x^2+8503056x+531441>0.
\end{aligned}\]
The proof is completed.
\end{proof}
\end{document}
