\documentclass[12pt,a4paper]{book}

\input{../template/standard_pkgs}
\input{../template/common}
\input{format}

\def\nvh{{\it Nguyễn Văn Huyện}}
\addto\captionsvietnam{\renewcommand{\proofname}{\cmss\problemColor Proof}}

\begin{document}
Setting $p=a+b+c,\,q=ab+bc+ca$ and $r=abc.$
\begin{pro}
Let $a,\,b,\,c$ are real numbers such that $p=1$ and $q>0.$ Prove that
\begin{equation}\label{eq1}
\frac{a}{a+b}+\frac{b}{b+c}+\frac{c}{c+a} \ge \frac{3}{2} - \frac{1}{2}\sqrt{\frac{(1-3q)^3}{q(q+1)^2}}.
\end{equation}
\end{pro}

\begin{proof} (\textit{Nguyen Van Huyen}) First, we will show that
\[pq-r = (a+b)(b+c)(c+a)>0.\]
Indeed, according to the AM-GM inequality, we have
\[0 < a(b+c)+bc \leqslant a(b+c)+\frac{(b+c)^2}{4}=a(1-a)+\frac{(1-a)^2}{4} = \frac{(1-a)(3a+1)}{4}.\]
Deduced $- \frac{1}{3} < a < 1,$ so $b+c=1-a>0,$ therefore
\[(a+b)(b+c)(c+a)>0.\]
Now, setting
\[M = \frac{3}{2} - \frac{1}{2}\sqrt{\frac{(1-3q)^3}{q(q+1)^2}},\]
We write the inequality \eqref{eq1} as
\[\frac{3(pq-r)-(a-b)(b-c)(c-a)}{pq-r} \geq 2M,\]
equivalent to
\[(3 - 2M)(pq-r) \ge (a-b)(b-c)(c-a),\]
Because
\[3 - 2M = \sqrt{\frac{(1-3q)^3}{q(q+1)^2}}>0,\]
so, we just need to prove that 
\[(3 - 2M)(pq-r) \ge \sqrt{(a-b)^2(b-c)^2(c-a)^2}.\]
or
\[(3 - 2M)(pq-r) \ge (a-b)^2(b-c)^2(c-a)^2.\]
This is equivalent to each of the following inequalities
\[(3 - 2M)^2(pq-r)^2 \ge q^2(p^2-4q)-2p(2p^2-9q)r-27r^2,\]
\[(3 - 2M)^2(q-r)^2 \ge q^2(1-4q)-2(2-9q)r-27r^2,\]
or
\[(M^2-3M+9)r^2-\big[(2M^2-6M+9)q-1\big]r+q^2(q+M^2-3M+2) \ge 0,\]
\[\frac{(9q+1)^2}{4q(q+1)^2} \cdot r^2 + \frac{(9q+1)(2q^2-5q+1)}{2(q+1)^2}\cdot r+\frac{q(2q^2-5q+1)^2}{4(q+1)^2} \ge 0,\]
or
\[\frac{\big[(9q+1)r+q(2q^2-5q+1)\big]^2}{4q(q+1)^2} \ge 0.\]
The proof is completed.
\end{proof}
\end{document}
