\documentclass[12pt,a4paper]{book}

\input{./template/standard_pkgs}
\input{./template/format}
\input{./template/define}

\begin{document}

\begin{pro_no_count}[Pham Kim Hung]
% https://artofproblemsolving.com/community/c6h57558
Let $a,\,b,\,c$ be non-negative numbers satisfying $a+b+c=2.$ Prove that
\begin{equation}\label{eq9}
\frac{bc}{a^2+1} + \frac{ca}{b^2+1} + \frac{ab}{c^2+1} \le 1.
\end{equation}
\end{pro_no_count}

\begin{proof}[\cmss\problemColor Solution 1]
(\textit{Vo Quoc Ba Can, Nguyen Van Huyen}) We have the following estimate
\begin{equation}\label{eq1}
\frac{bc}{a^2+1} \le \frac{bc(b+c)}{ab(a+b)+bc(b+c)+ca(c+a)}.
\end{equation} 
If $bc = 0,$ then \eqref{eq1} is obvious.

If $bc >0,$ dividing both sides by $bc$ and homogenizing the inequality becomes
\[[4a^2+(a+b+c)^2](b+c) \geq  4[a b(a+b)+b c(b+c)+c a(c+a)].\]
The inequality is quadratic in $a,$ so we can rewrite it as
\[(b+c)a^2-2a(b-c)^2+(b+c)(b-c)^2 \ge 0,\]
or
\[(b+c)[a^2+(b-c)^2] \ge 2a(b-c)^2.\]
Since $b+c \ge |b-c|,$ using the AM-GM inequality, we have
\[(b+c)[a^2+(b-c)^2] \ge (b+c) \cdot  2a \cdot |b-c| = 2a(b+c)|b-c| \ge 2a(b-c)^2.\]
Thus
\[\sum \frac{bc}{a^2+1} \le \sum \frac{bc(b+c)}{ab(a+b)+bc(b+c)+ca(c+a)} = 2.\]
The equality holds for $a=0, \ b = c = 1$ (or any cyclic permutation).
\end{proof}

\begin{proof}[\cmss\problemColor Solution 2]
(\textit{Nguyen Van Huyen}) We have the following estimate
\[\frac{bc}{a^2+1} \leqslant \frac{a^2+b^2+c^2-2a(b+c)+6bc}{3(a^2+b^2+c^2)+2(ab+bc+ca)}.\]
Indeed, since
\[[a^2+b^2+c^2-2a(b+c)+6bc]\left[a^2+\frac{1}{4}(a+b+c)^2\right] - bc[3(a^2+b^2+c^2)+2(ab+bc+ca)]\]
\[=a^2(b+c-a)^2+\frac{1}{4}(a+b-c)^2(c+a-b)^2 \geqslant 0.\]
We have
\[\frac{bc}{a^2+\frac{(a+b+c)^2}{4}} \leqslant \frac{a^2+b^2+c^2-2a(b+c)+6bc}{3(a^2+b^2+c^2)+2(ab+bc+ca)},\]
or
\[\frac{bc}{a^2+1} \leqslant \frac{a^2+b^2+c^2-2a(b+c)+6bc}{3(a^2+b^2+c^2)+2(ab+bc+ca)}.\]
% Thus
% \[\sum \frac{bc}{a^2+1} \le \sum \frac{a^2+b^2+c^2-2a(b+c)+6bc}{3(a^2+b^2+c^2)+2(ab+bc+ca)} = 1.\]
\end{proof}

\begin{note}
From this solution, we see that \eqref{eq9} is always true for all \textbf{\textit{real}} numbers.
\end{note}

\end{document}
