\documentclass[12pt,a4paper]{book}

\input{./template/standard_pkgs}
\input{./template/common}
\input{./template/format}

\begin{document}
\begin{pro}
Let $a,\,b,\,c$ be three positive real numbers. Prove that
\[(a+b+c-3)\left(\frac{1}{a}+\frac{1}{b}+\frac{1}{c}-3\right)+abc+\frac{1}{abc} \geqslant 2.\]
\begin{flushright}(Nguyen Van Huyen)\end{flushright}
\end{pro}

\begin{proof}[\cmss\problemColor Solution] (\textit{Nguyen Van Huyen}) We rewrite the inequality as
\[(a+b+c-3)(ab+bc+ca-3abc)+a^2b^2c^2+1 \geqslant 2abc.\]
Group the inequality as a quadratic in terms of $a$
\[(b^2c^2+b+c-3bc)a^2 - [b^2+10bc+c^2 - 3(b+c)(1+bc)]a + bc(b+c) - 3bc + 1 \ge 0.\]
By the AM-GM inequality, we have
% \[b^2c^2-3bc+b+c \ge b^2c^2-3bc+2\sqrt{bc}=t^4-3t^2+2t=t(t+2)(t-1)^2  \geqslant 0.\]
\[b^2c^2+b+c \geqslant 3\sqrt[3]{b^2c^2 \cdot b \cdot c} = 3bc,\]
\[bc(b+c) + 1 \geqslant 3\sqrt[3]{b^2c \cdot bc^2 \cdot 1} = 3bc.\]
We consider two cases
\begin{enumerate}[(1)]
\item If $b^2+10bc+c^2 > 3(b+c)(1+bc),$ then it is obvious.
\item If $b^2+10bc+c^2 \le 3(b+c)(1+bc),$ we calculate the discriminant
\[\begin{aligned}
\Delta &= \big[b^2+10bc+c^2 - 3(b+c)(1+bc)\big]^2 - 4(b^2c^2+b+c-3bc)[bc(b+c) - 3bc + 1] \\
&= -(b-1)^2(c-1)^2[4(b+c)(bc+1) - b^2-14bc-c^2] \\
%&= -\frac13(b-1)^2(c-1)^2\big[4[3(b+c)(1+bc)-(b^2+10bc+c^2)]+(b-c)^2\big] \\
\end{aligned}\]
Since 
%\[4(b+c)(bc+1) - b^2-14bc-c^2 = 4[3(b+c)(1+bc)-b^2-10bc-c^2]+(b-c)^2 \ge 0.\]
\[\begin{aligned}
4(b+c)(bc+1) &- b^2-14bc-c^2 \\&= \frac{4[3(b+c)(1+bc)-b^2-10bc-c^2]}{3}+\frac{(b-c)^2}{3} \ge 0.
\end{aligned}\] 
We obtain $\Delta \le 0.$
\end{enumerate}
The proof completed.
\end{proof}

\section*{References}

\begin{enumerate}[label={[\arabic*]}]
\item \href{https://artofproblemsolving.com/community/c6h3460563p33432469}{\url{https://artofproblemsolving.com/community/c6h3460563p33432469}}
\end{enumerate}

\end{document}
